refocusing_examples/lam_ses_no.v
@@ -323,7 +323,7 @@ Module Lam_SES_NO_PreRefSem <: PRE_PRECISE_REF_SEM.
     | |- App (valCa_to_term ?v) _ <> _ => dependent_destruction2 v
     end;
     destruct_all sub_tag; destruct_all substitut;
-      
+
     solve [ discriminate | tauto ].
   Qed.
 
@@ -358,7 +358,7 @@ Module Lam_SES_NO_PreRefSem <: PRE_PRECISE_REF_SEM.
 
     solve (*rest with*)
     [ destruct_all sub_tag; destruct_all substitut;
-      inversion H1; subst; 
+      inversion H1; subst;
       auto ].
   Qed.
 
@@ -589,14 +589,14 @@ Module Lam_SES_NO_Strategy <: REF_STRATEGY Lam_SES_NO_PreRefSem.
   Proof. REF_LANG_Help.prove_ec_wf. Qed.
 
 
-  Lemma search_order_antisym : forall k t ec ec0, 
+  (*Lemma search_order_antisym : forall k t ec ec0, 
       k, t |~ ec << ec0 -> ~ k, t |~ ec0 << ec.
 
   Proof.
     intros k t ec ec0 H.
     destruct k, ec, ec0;
     solve [ autof ].
-  Qed.
+  Qed.*)
 
 
   Lemma search_order_trans :  forall k t ec0 ec1 ec2, 
